theories/TM/Reductions/mTM_to_TM.v
@@ -1,6 +1,9 @@
 From Undecidability.TM Require Import Single.StepTM Code.CodeTM TM.
 Require Import Undecidability.Synthetic.Definitions.
 
+Set Default Goal Selector "!".
+Set Default Proof Using "Type".
+
 Lemma nTM_to_MTM n :
   HaltTM n ⪯ HaltMTM.
 Proof.
@@ -13,46 +16,67 @@ Qed.
 
 Lemma mk_pTM n (sig : finType) (m : TM sig n) : pTM sig unit n.
 Proof.
-  unshelve econstructor. exact m. exact (fun _ => tt).
+  unshelve econstructor.
+  - exact m.
+  - exact (fun _ => tt).
 Defined. (* because definition *)
 
 Local Notation "[ s | p ∈ A ]" := (map (fun p => s) A) (p pattern).
+
+Section MTM_to_stM.
+
+Variables (n : nat) (sig : finType) (M : TM sig n) (ts : Vector.t (tape sig) n).
+
+Definition sig' := (sigList (EncodeTapes.sigTape sig)) ^+.
+Definition M' : TM sig' 1.
+Proof using M.
+  eapply mk_pTM in M.
+  destruct (ToSingleTape M) as [M' HM'].
+  exact M'.
+Defined.
+
+Definition ts' : Vector.t (tape sig') 1.
+Proof using ts.
+  eapply EncodeTapes.encode_tapes in ts.
+  pose (midtape nil (inl START) (map inr ts ++ [inl STOP])) as t'.
+  exact (Vector.cons _ t' _ (Vector.nil _)).
+Defined.
+
+Lemma MTM_to_stM_correct : HaltsTM M ts <-> HaltsTM M' ts'.
+Proof.
+  unfold HaltsTM, M'. setoid_rewrite TM_eval_iff.
+  split; intro H.
+  + destruct H as (q' & t' & k & H).
+    assert (M ↓ (fun t' k' => ts = t' /\ k' = k)) as H0.
+    { intros ? ? []. subst. eauto. }
+    eapply (ToSingleTape_Terminates' (pM := mk_pTM M)) in H0.
+    specialize (H0 [|midtape [] (inl START) ([inr p | p ∈ EncodeTapes.encode_tapes ts] ++ [inl STOP])|]).
+    edestruct H0 as [x H1].
+    * exists ts, k. repeat split; eauto.
+    * destruct x as [q'' t'']. exists q'', t''. 
+      destruct ((ToSingleTape (mk_pTM M))).
+      eexists.
+      eapply H1.
+  + destruct H as (q' & t' & k & H). cbn in *.
+    pose proof (ToSingleTape_Realise' (pM := mk_pTM M)) as H0.
+    specialize (H0 (fun t '(f,t') => exists outc k, loopM (initc M t) k = Some outc /\ ctapes outc = t')).
+    edestruct H0 as [d [H2 ?] c dd].
+    * intros ? k0 outc ?. exists outc, k0. eauto.
+    * eapply H.
+    * firstorder easy.
+    * destruct H2 as (x0 & x1 & ? & ?). subst.
+      destruct x0 as [q'' t''].
+      now exists q'', t'', x1.
+Qed.
+
+End MTM_to_stM.
 
 Lemma MTM_to_stM :
   HaltMTM ⪯ HaltTM 1.
 Proof.
   unshelve eexists.
-  - intros [ [n sig] M t].
-    eapply mk_pTM in M. 
-    pose (ToSingleTape M). cbn in *.
-    eexists. destruct p. exact x.
-    cbn.
-    eapply EncodeTapes.encode_tapes in t.
-    econstructor. 2:econstructor.
-    refine (midtape nil (inl START) (map inr t ++ [inl STOP])).
-  - intros [ [n sig] M t]. cbn.
-    unfold HaltsTM.
-    setoid_rewrite TM_eval_iff.
-    intuition.
-    + destruct H as (q' & t' & k & H).
-      assert (M ↓ (fun t' k' => t = t' /\ k' = k)).
-      { intros ? ? []. subst. eauto. }
-      eapply (ToSingleTape_Terminates' (pM := mk_pTM M)) in H0.
-      specialize (H0 [|midtape [] (inl START) ([inr p | p ∈ EncodeTapes.encode_tapes t] ++ [inl STOP])|]).
-      edestruct H0. 
-      * exists t, k. repeat split; eauto.
-      * destruct x as [q'' t'']. exists q'', t''. 
-        destruct ((ToSingleTape (mk_pTM M))).
-        eexists.
-        eapply H1.
-    + destruct H as (q' & t' & k & H). cbn in *.
-      pose proof (ToSingleTape_Realise' (pM := mk_pTM M)).
-      specialize (H0 (fun t '(f,t') => exists outc k, loopM (initc M t) k = Some outc /\ ctapes outc = t')).
-      edestruct H0.
-      * intros ? ? ? ?. exists outc, k0. eauto.
-      * eapply H.
-      * firstorder.
-      * intuition. destruct H2 as (? & ? & ? & ?). subst.
-        destruct x0 as [q'' t''].
-        now exists q'', t'', x1.
+  { intros [[n sig] M ts].
+    exact (existT2 _ _ (sig' sig) (M' M) (ts' ts)). }
+  intros [[n sig] M ts].
+  apply MTM_to_stM_correct.
 Qed.
