theories/TM/TM_undec.v
@@ -2,7 +2,6 @@ Require Import Undecidability.Synthetic.Undecidability.
 Require Import Undecidability.Synthetic.ReducibilityFacts.
 Require Import Undecidability.TM.TM.
 
-Require Import Undecidability.TM.Reductions.mTM_to_TM.
 Require Import Undecidability.TM.Reductions.SBTM_HALT_to_HaltTM_1.
 Require Import Undecidability.TM.SBTM_undec.
 (** ** HaltMTM and HaltTM 1 are undecidable *)
@@ -12,7 +11,9 @@ Lemma HaltMTM_undec :
 Proof.
   apply (undecidability_from_reducibility SBTM_HALT_undec).
   apply (reduces_transitive SBTM_HALT_to_HaltTM_1.reduction).
-  apply nTM_to_MTM.
+  unshelve eexists.
+  - intros [Sig M t]. exists (1, Sig); eassumption.
+  - now intros [Sig M t].
 Qed.
 
 Lemma HaltTM_1_undec :
