theories/TM/UTM_undec.v
@@ -1,0 +1,14 @@
+From Undecidability Require Import
+  Synthetic.Undecidability Synthetic.ReducibilityFacts
+  LambdaCalculus.Krivine_undec TM.UTM.
+
+From Undecidability Require TM.Reductions.KrivineMclosed_HALT_to_HaltUTM.
+
+(** ** HaltUTM is undecidable *)
+
+Lemma HaltUTM_undec :
+  undecidable HaltUTM.
+Proof.
+  apply (undecidability_from_reducibility KrivineMclosed_HALT_undec).
+  exact KrivineMclosed_HALT_to_HaltUTM.reduction.
+Qed.
