README.md
@@ -43,7 +43,7 @@ Target problems are very expressive and thus work well as targets for reduction,
 - Halting problem for the weak call-by-value lambda-calculus (`HaltL` in [`L/L.v`](theories/L/L.v))
 - Halting problem for multi-tape Turing machines (`HaltMTM` in [`TM/TM.v`](theories/TM/TM.v))
 - Halting problem for single-tape Turing machines (`HaltTM 1` in [`TM/TM.v`](theories/TM/TM.v))
-- Halting problem for simple binary single-tape Turing machines (`HaltSBTM` in [`TM/SBTM.v`](theories/TM/SBTM.v))
+- Halting problem for simple binary single-tape Turing machines (`SBTM_HALT`) in [`TM/SBTM.v`](theories/TM/SBTM.v)
 - Halting problem for program counter based binary single-tape Turing machines (`PCTM_HALT` in [`TM/PCTM.v`](theories/TM/PCTM.v))
 - Halting problem for Binary Stack Machines (`BSM_HALTING` in [`StackMachines/BSM.v`](theories/StackMachines/BSM.v))
 - Halting problems for Minsky machines (`MM_HALTING` and `MMA_HALTING n` in [`MinskyMachines/MM.v`](theories/MinskyMachines/MM.v))
